 @prefix dc: <http://purl.org/dc/terms/> .
@prefix dcterms: <http://purl.org/dc/terms/> .
@prefix rdf: <http://www.w3.org/1999/02/22-rdf-syntax-ns#> .
@prefix rdfs: <http://www.w3.org/2000/01/rdf-schema#> .
@prefix schema: <http://schema.org/> .
@prefix xml: <http://www.w3.org/XML/1998/namespace> .
@prefix xsd: <http://www.w3.org/2001/XMLSchema#> .

schema:BasicData a rdfs:Class ;
    rdfs:label "BasicData" ;
    dc:source <http://vocab.datex.org/terms#BasicData> ;
    schema:isPartOf <http://mobility.schema.org> ;
    rdfs:comment "Data that is either measured or calculated (elaborated) at the same time or over the same time period. " ;
    rdfs:subClassOf schema:QuantitativeValue .

schema:Environment a rdfs:Class ;
    rdfs:label "Environment" ;
    schema:isPartOf <http://mobility.schema.org> ;
    rdfs:comment "An Environment category class." ;
    rdfs:subClassOf schema:Enumeration .

schema:Parking a rdfs:Class ;
    rdfs:label "Parking" ;
    schema:isPartOf <http://mobility.schema.org> ;
    rdfs:comment "A Parking category class." ;
    rdfs:subClassOf schema:Enumeration .

schema:ParkingSite a rdfs:Class ;
    rdfs:label "Parking Site" ;
    dc:source <http://vocab.datex.org/terms#ParkingSite> ;
    schema:isPartOf <http://mobility.schema.org> ;
    rdfs:comment "A parking site." ;
    rdfs:subClassOf schema:ParkingFacility .

schema:ParkingSiteStatus a rdfs:Class ;
    rdfs:label "Parking Site Status" ;
    dc:source <http://vocab.datex.org/terms#ParkingSiteStatus> ;
    schema:isPartOf <http://mobility.schema.org> ;
    rdfs:comment "Status of a parking site." ;
    rdfs:subClassOf schema:QuantitativeValue .

schema:ParkingSpace a rdfs:Class ;
    rdfs:label "Parking Space" ;
    dc:source <http://vocab.datex.org/terms#ParkingSpace> ;
    schema:isPartOf <http://mobility.schema.org> ;
    rdfs:comment """A single parking space. It is possible to define the same parking space more than once with different properties, 
		e.g. when there is a different parking assignment for different times.""";
    rdfs:subClassOf schema:ParkingFacility .

schema:ParkingSpaceStatus a rdfs:Class ;
    rdfs:label "ParkingSpaceStatus" ;
    dc:source <http://vocab.datex.org/terms#ParkingSapceStatus> ;
    schema:isPartOf <http://mobility.schema.org> ;
    rdfs:comment "Current status of a parking space." ;
    rdfs:subClassOf schema:Enumeration .

schema:TpegAreaLocation a rdfs:Class ;
    rdfs:label "tpeg area location" ;
    dc:source <http://vocab.datex.org/terms#TpegAreaLocation> ;
    schema:isPartOf <http://mobility.schema.org> ;
    rdfs:comment "A geographic or geometric area defined by a TPEG-Loc structure which may include height information for additional geospatial discrimination." ;
    rdfs:subClassOf schema:Thing .

schema:TpegGeometricArea a rdfs:Class ;
    rdfs:label "TpegGeometricArea" ;
    dc:source <http://vocab.datex.org/terms#TpegGeometricArea> ;
    schema:isPartOf <http://mobility.schema.org> ;
    rdfs:comment "A geometric area defined by a centre point and a radius." ;
    rdfs:subClassOf schema:TpegAreaLocation .

schema:TpegLinearLocation a rdfs:Class ;
    rdfs:label "tpeg linear location" ;
    dc:source <http://vocab.datex.org/terms#TpegLinearLocation> ;
    schema:isPartOf <http://mobility.schema.org> ;
    rdfs:comment "A linear section along a single road defined between two points on the same road by a TPEG-Loc structure." ;
    rdfs:subClassOf schema:Thing .

schema:Traffic a rdfs:Class ;
    rdfs:label "Traffic" ;
    schema:isPartOf <http://mobility.schema.org> ;
    rdfs:comment "A Traffic category class." ;
    rdfs:subClassOf schema:Enumeration .

schema:TrafficData a rdfs:Class ;
    rdfs:label "TrafficData" ;
    dc:source <http://vocab.datex.org/terms#TrafficData> ;
    schema:isPartOf <http://mobility.schema.org> ;
    rdfs:comment "Measured or derived values relating to traffic or individual vehicle movements on a specific section or at a specific point on the road network." ;
    rdfs:subClassOf schema:BasicData .

schema:TrafficSpeed a rdfs:Class ;
    rdfs:label "TrafficSpeed" ;
    dc:source <http://vocab.datex.org/terms#TrafficSpeed> ;
    schema:isPartOf <http://mobility.schema.org> ;
    rdfs:comment "Averaged measurements or calculations of traffic speed." ;
    rdfs:subClassOf schema:TrafficData .

schema:Transportation a rdfs:Class ;
    rdfs:label "Transportation" ;
    schema:isPartOf <http://mobility.schema.org> ;
    rdfs:comment "A Transportation category class." ;
    rdfs:subClassOf schema:Enumeration .

schema:TravelTimeData a rdfs:Class ;
    rdfs:label "TravelTimeData" ;
    dc:source <http://vocab.datex.org/terms#TravelTimeData> ;
    schema:isPartOf <http://mobility.schema.org> ;
    rdfs:comment "Derived/computed travel time information relating to a linear section of the road network; forecast = true means a forecast for a vehicle at the start of the specified location, forecast = false means calculation/measurement at the end." ;
    rdfs:subClassOf schema:BasicData .

schema:busTransportation a schema:Transportation ;
    rdfs:label "busTransportation" ;
    rdfs:comment "A sub-category of Transportation to categorize the things relating to bus transportation." .

schema:carTransportation a schema:Transportation ;
    rdfs:label "carTransportation" ;
    rdfs:comment "A sub-category of Transportation to categorize the things relating to car transportation." .

schema:distanceFromParkingSpace a rdf:Property ;
    rdfs:label "distanceFromParkingSpace" ;
    dc:source <http://vocab.datex.org/terms#distanceFromParkingSpace> ;
    schema:domainIncludes schema:ParkingSpace ;
    schema:isPartOf <http://mobility.schema.org> ;
    schema:rangeIncludes schema:Number ;
    rdfs:comment "distance from parking space" .

schema:environment a schema:Environment ;
    rdfs:label "traffic" ;
    rdfs:comment "A environment category." .

schema:from a rdf:Property ;
    rdfs:label "from" ;
    schema:domainIncludes schema:TpegLinearLocation ;
    schema:isPartOf <http://mobility.schema.org> ;
    schema:rangeIncludes schema:GeoCoordinates ;
    rdfs:comment "The location at the up stream end of the section of road which frames the TPEGFramedPoint." .

schema:hasGeoShape a rdf:Property ;
    rdfs:label "hasGeoShape" ;
    schema:domainIncludes schema:TpegGeometricArea ;
    schema:isPartOf <http://mobility.schema.org> ;
    schema:rangeIncludes schema:GeoCircle ;
    rdfs:comment "Geoshape of the TpegGeometricArea." .

schema:hasParkingSapceOrGroupIdentifier a rdf:Property ;
    rdfs:label "parkingSapceOrGroupIdentifier" ;
    dc:source <http://vocab.datex.org/terms#parkingSpaceOrGroupIdentifier> ;
    schema:domainIncludes schema:ParkingSite,
        schema:ParkingSpace ;
    schema:isPartOf <http://mobility.schema.org> ;
    schema:rangeIncludes schema:Text,
        schema:Url ;
    rdfs:comment "A property that relates parking site or space with parking identifier" .

schema:occupiedSpaceAppeared a schema:ParkingSpaceStatus ;
    rdfs:label "occupiedSpaceAppeared" ;
    dc:source <http://vocab.datex.org/terms#occupiedSpaceAppeared> ;
    rdfs:comment "occupied parking space appeared." .

schema:occupiedSpaceDisappeared a schema:ParkingSpaceStatus ;
    rdfs:label "occupiedSpaceDisappeared" ;
    dc:source <http://vocab.datex.org/terms#occupiedSpaceDisappeared> ;
    rdfs:comment "occupied parking space disappeared." .

schema:parking a schema:Parking ;
    rdfs:label "parking" ;
    rdfs:comment "A parking category." .

schema:parkingLocation a rdf:Property ;
    rdfs:label "parkingLocation" ;
    dc:source <http://vocab.datex.org/terms#parkingLocation> ;
    schema:domainIncludes schema:ParkingSpace ;
    schema:isPartOf <http://mobility.schema.org> ;
    schema:rangeIncludes schema:GeoCoordinates ;
    rdfs:comment "Location or geo coordinates of a parking space" .

schema:parkingNumberOfOccupiedSpaces a rdf:Property ;
    rdfs:label "parkingNumberOfOccupiedSpaces" ;
    dc:source <http://vocab.datex.org/terms#parkingNumberOfOccupiedSpaces> ;
    schema:domainIncludes schema:ParkingSiteStatus ;
    schema:isPartOf <http://mobility.schema.org> ;
    schema:rangeIncludes schema:Number ;
    rdfs:comment "parking number of occupied spaces" .

schema:parkingNumberOfVacantSpaces a rdf:Property ;
    rdfs:label "parkingNumberOfVacantSpaces" ;
    dc:source <http://vocab.datex.org/terms#parkingNumberOfVacantSpaces> ;
    schema:domainIncludes schema:ParkingSiteStatus ;
    schema:isPartOf <http://mobility.schema.org> ;
    schema:rangeIncludes schema:Number ;
    rdfs:comment "parking number of vacant spaces" .

schema:parkingSapceStatus a rdf:Property ;
    rdfs:label "parkingSapceStatus" ;
    dc:source <http://vocab.datex.org/terms#parkingSapceStatus> ;
    schema:domainIncludes schema:ParkingSpace ;
    schema:isPartOf <http://mobility.schema.org> ;
    schema:rangeIncludes schema:ParkingSpaceStatus ;
    rdfs:comment "A property that relates parking space with its current status" .

schema:parkingSiteManagement a schema:Parking ;
    rdfs:label "parkingSiteMgmtCategory" ;
    rdfs:comment "A sub-category of Parking to categorize the things relating to parking site management." .

schema:parkingSiteStatus a rdf:Property ;
    rdfs:label "parkingSiteStatus" ;
    dc:source <http://vocab.datex.org/terms#parkingSiteStatus> ;
    schema:domainIncludes schema:ParkingSite ;
    schema:isPartOf <http://mobility.schema.org> ;
    schema:rangeIncludes schema:ParkingSiteStatus ;
    rdfs:comment "The status of the parking site " .

schema:parkingSpaceManagement a schema:Parking ;
    rdfs:label "parkingSpaceMgmtCategory" ;
    rdfs:comment "A sub-category of Parking to categorize the things relating to parking space management." .

schema:parkingSpaceStatusTimeStamp a rdf:Property ;
    rdfs:label "parkingSpaceStatusTimeStamp" ;
    schema:domainIncludes schema:ParkingSpace ;
    schema:isPartOf <http://mobility.schema.org> ;
    schema:rangeIncludes schema:DateTime ;
    rdfs:comment "Timestamp when the status of the parking space has last changed" .

schema:potentialSpaceAppeared a schema:ParkingSpaceStatus ;
    rdfs:label "potentialSpaceAppeared" ;
    dc:source <http://vocab.datex.org/terms#potentialSpaceAppeared> ;
    rdfs:comment "potential parking space appeared." .

schema:potentialSpaceDisappeared a schema:ParkingSpaceStatus ;
    rdfs:label "potentialSpaceDisappeared" ;
    dc:source <http://vocab.datex.org/terms#potentialSpaceDisappeared> ;
    rdfs:comment "potential parking space disappeared." .

schema:speed a rdf:Property ;
    rdfs:label "traffic speed" ;
    schema:domainIncludes schema:TrafficSpeed ;
    schema:isPartOf <http://mobility.schema.org> ;
    schema:rangeIncludes schema:Number ;
    rdfs:comment "A value of speed expressed in kilometres per hour." .

schema:to a rdf:Property ;
    rdfs:label "to" ;
    schema:domainIncludes schema:TpegLinearLocation ;
    schema:isPartOf <http://mobility.schema.org> ;
    schema:rangeIncludes schema:GeoCoordinates ;
    rdfs:comment "The location at the down stream end of the section of road which frames the TPEGFramedPoint." .

schema:totalCapacity a rdf:Property ;
    rdfs:label "totalCapacity" ;
    dc:source <http://vocab.datex.org/terms#totalCapacity> ;
    schema:domainIncludes schema:ParkingSite ;
    schema:isPartOf <http://mobility.schema.org> ;
    schema:rangeIncludes schema:Number ;
    rdfs:comment "Total number of car parking spaces" .

schema:tpegAreaDescriptor a rdf:Property ;
    rdfs:label "tpegAreaDescriptor" ;
    schema:domainIncludes schema:TpegGeometricArea ;
    schema:isPartOf <http://mobility.schema.org> ;
    schema:rangeIncludes schema:Text ;
    rdfs:comment "Name of area." .

schema:traffic a schema:Traffic ;
    rdfs:label "traffic" ;
    rdfs:comment "A traffic category." .

schema:trafficInformation a schema:Traffic ;
    rdfs:label "trafficInformationCategory" ;
    rdfs:comment "A sub-category of Traffic to categorize the things relating to bus traffic information." .

schema:trafficMonitoring a schema:Traffic ;
    rdfs:label "trafficMonitoringCategory" ;
    rdfs:comment "A sub-category of Traffic to categorize the things relating to Traffic monitoring." .

schema:transportation a schema:Transportation ;
    rdfs:label "transportation" ;
    rdfs:comment "A transportation category." .

schema:travelTime a rdf:Property ;
    rdfs:label "travel time" ;
    schema:domainIncludes schema:TravelTimeData ;
    schema:isPartOf <http://mobility.schema.org> ;
    schema:rangeIncludes schema:Time ;
    rdfs:comment "Derived/computed travel time information relating to a specific group of locations." .


